\documentclass{article}
\usepackage{german}
\setlength{\textwidth}{135mm}
\begin{document}
\noindent
Laurent-Entwicklung:  Mit $c_n = \frac{1}{2\pi i}
\oint (\zeta-a)^{-n-1}f(\zeta)\,d\zeta$ gilt f"ur jede Funk\-tion $f(z)$ die
Darstellung ($n=0$, $\pm1$, $\pm2$, \ldots)
\[ f(x) = \sum_{n=-\infty}^{+\infty} c_n(z-a)^n
	= \left\{\begin{array}{r}
	  c_0 + c_1(z-a) + c_2(z-a)^2 +\cdots+ c_n(z-a)^n+\cdots\\
	  \mbox{}+c_{-1}(z-a)^{-1} + c_{-2}(z-a)^{-2}+\cdots\\
	  \mbox{}+c_{-n}(z-a)^{-n}+\cdots \end{array}\right. \]
\end{document}
